theories/RTL/SimRules.v
@@ -1,11 +1,9 @@
-From RSL Require Import Prelude.
+From RSL Require Import Prelude RelLogic.
 
 From Coinduction Require Import all.
 
-From RSL Require Import Commons.Bilogic.
-From RSL Require Import Commons.Logic.
-
 From RSL Require Import Simulations.FreeSim.
+From RSL Require Import Simulations.FreeSimRules.
 
 From RSL Require Import RTL.RTL.
 From RSL Require Import RTL.Semantics.
@@ -16,117 +14,240 @@ Import RTLNotations.
 Section Rules.
   Let Λₜ : lang := rtl_lang.
   Let Λₛ : lang := rtl_lang.
-  Context (Pₜ: prog Λₜ) (Pₛ: prog Λₛ) (Φ: val -> val -> memory -> memory -> Prop).
+  Context (Pₜ: prog Λₜ) (Pₛ: prog Λₛ).
 
-  Definition sim Φ (stepₜ: nat) '(fₜ, pcₜ) (stepₛ: nat) '(fₛ, pcₛ) : bilogic :=
-    let Φ := fun '(vₜ, mₜ) '(vₛ, mₛ) => Φ vₜ vₛ mₜ mₛ in
-    fun '(ρₜ, mₜ) '(ρₛ, mₛ) =>
-      gfp (fsim_lfp _ _ Pₜ Pₛ Φ) stepₜ ([], State fₜ pcₜ ρₜ, mₜ) stepₛ ([], State fₛ pcₛ ρₛ, mₛ).
+  Abbreviation fsim := (fsim WfNat WfNat Pₜ Pₛ).
+  Abbreviation fsim_lfp := (fsim_lfp WfNat WfNat Pₜ Pₛ).
+  Abbreviation rlogic := (rlogic _ _).
 
-  Hint Unfold sim : custom_bilogic.
+  Definition sim GFP Q (stepₜ: nat) fₜ pcₜ (stepₛ: nat) fₛ pcₛ : rlogic :=
+    let sim_rtl Φ : rlogic :=
+      (fun ρₜ ρₛ mₜ mₛ =>
+         fsim_lfp GFP Φ
+           stepₜ ([], State fₜ pcₜ ρₜ, mₜ)
+           stepₛ ([], State fₛ pcₛ ρₛ, mₛ))
+    in
+    ⦇ ∀ Φ,
+        ⌜∀ vₜ vₛ mₜ mₛ, Q vₜ vₛ mₜ mₛ -> Φ (vₜ, mₜ) (vₛ, mₛ)⌝ ->
+        sim_rtl Φ ⦈.
 
-  Notation "t '⟨' iₜ '≲' iₛ '⟩' s '{{' Φ '}}'" :=
-    (sim Φ iₜ t iₛ s)
-      (at level 1, no associativity).
+  Notation
+    "C ⊢ '⟨' ft '@' pct ',' j '⟩' '≲' '⟨' fs '@' pcs ',' i '⟩' '{{' Φ '}}'" :=
+    (sim (elem C) Φ j ft pct i fs pcs)
+      (at level 1, ft at level 0, fs at level 0, no associativity).
 
-  Lemma source_nop iₜ iₛ fₜ fₛ pcₜ pcₛ : ∀ pc,
-    fₛ@pcₛ is <{ nop -> pc }> ->
-    ⊨ (fₜ, pcₜ) ⟨iₜ ≲ S iₛ⟩ (fₛ, pc) {{ Φ }} ->
-    (fₜ, pcₜ) ⟨iₜ ≲ iₛ⟩ (fₛ, pcₛ) {{ Φ }}.
+  Lemma both_ret (C : Chain fsim_lfp) Q j fₜ pcₜ i fₛ pcₛ :
+    ∀ rₜ vₜ rₛ vₛ,
+    fₜ@pcₜ is <{ ret rₜ }> ->
+    fₛ@pcₛ is <{ ret rₛ }> ->
+    ⊨ rₜ ⇒ₜ vₜ ->
+      rₛ ⇒ₛ vₛ ->
+      ⌜Q vₜ vₛ⌝ₘ ->
+      C ⊢ ⟨fₜ @ pcₜ, j⟩ ≲ ⟨fₛ @ pcₛ, i⟩ {{ Q }}.
   Proof using Type.
-    intros pc Hpc [ρₜ mₜ] [ρₛ mₛ] H.
-    unfold_bilogic.
-    apply (@fsim_roll Λₜ Λₛ).
-    eapply FSourceSteps.
-    - constructor; eassumption.
-    - eapply (@fsim_unroll Λₜ Λₛ).
-      apply H.
+    intros rt vt rs vs Hpct Hpcs.
+    intros ρₜ ρₛ mₜ mₛ Ht Hs HQ Ψ Hpost. simp.
+    eapply FSourceSteps with (i' := 0).
+    { econstructor; eassumption || reflexivity. }
+    eapply FTargetSteps.
+    { eexists; econstructor; eassumption || reflexivity. }
+    intros t' Hstep. inv Hstep.
+    exists 0.
+    eapply FBothFinal.
+    do 2 econstructor. repeat split.
+    now apply Hpost.
   Qed.
 
-  Lemma target_nop iₜ iₛ fₜ fₛ pcₜ pcₛ : ∀ pc,
-    fₜ@pcₜ is <{ nop -> pc }> ->
-    ⊨ (fₜ, pc) ⟨S iₜ ≲ iₛ⟩ (fₛ, pcₛ) {{ Φ }} ->
-    (fₜ, pcₜ) ⟨iₜ ≲ iₛ⟩ (fₛ, pcₛ) {{ Φ }}.
+  Lemma source_nop (C : Chain fsim_lfp) Q j fₜ pcₜ i fₛ pcₛ :
+    ∀ pc,
+    fₛ@pcₛ is <{ nop -> pc }> ->
+    ⊨ C ⊢ ⟨fₜ @ pcₜ, j⟩ ≲ ⟨fₛ @ pc, S i⟩ {{ Q }} ->
+      C ⊢ ⟨fₜ @ pcₜ, j⟩ ≲ ⟨fₛ @ pcₛ, i⟩ {{ Q }}.
   Proof using Type.
-    intros pc Hpc [ρₜ mₜ] [ρₛ mₛ] H.
-    unfold_bilogic.
-    apply (@fsim_roll Λₜ Λₛ).
+    intros pc Hpc.
+    intros ρₜ ρₛ mₜ mₛ H Ψ Hpost. simp.
+    eapply FSourceSteps.
+    - constructor; eassumption.
+    - now apply H.
+  Qed.
+
+  Lemma target_nop (C : Chain fsim_lfp) Q j fₜ pcₜ i fₛ pcₛ :
+    ∀ pc,
+    fₜ@pcₜ is <{ nop -> pc }> ->
+    ⊨ C ⊢ ⟨fₜ @ pc, S j⟩ ≲ ⟨fₛ @ pcₛ, i⟩ {{ Q }} ->
+      C ⊢ ⟨fₜ @ pcₜ, j⟩ ≲ ⟨fₛ @ pcₛ, i⟩ {{ Q }}.
+  Proof using Type.
+    intros pc Hpc.
+    intros ρₜ ρₛ mₜ mₛ H Ψ Hpost. simp.
     eapply FTargetSteps.
     - eexists. constructor; eassumption.
     - intros t Hstep. inv Hstep.
-      eexists.
-      eapply (@fsim_unroll Λₜ Λₛ).
-      apply H.
+      eexists. now apply H.
   Qed.
 
-  Lemma source_op iₜ iₛ fₜ fₛ pcₜ pcₛ :
+  Lemma mapMtoMap {A B : Type} : ∀ (f : A -> B) args,
+    mapM (fun x => Some (f x)) args = Some (map f args).
+  Proof using Type.
+    intros f args.
+    induction args as [ | hd tl IH ].
+    - reflexivity.
+    - simpl. now rewrite IH.
+  Qed.
+
+  Lemma source_op (C : Chain fsim_lfp) Q j fₜ pcₜ i fₛ pcₛ :
     ∀ pc dst op regs args v,
     fₛ@pcₛ is <{ dst := @op regs -> pc }> ->
     eval_op op args = Some v ->
-    ⊨ regs ↪ₛ args ->
-      ⟦ dst ↩ₛ v ⟧ (fₜ, pcₜ) ⟨iₜ ≲ S iₛ⟩ (fₛ, pc) {{ Φ }} ->
-      (fₜ, pcₜ) ⟨iₜ ≲ iₛ⟩ (fₛ, pcₛ) {{ Φ }}.
+    ⊨ regs ⇒ₛ args ->
+      ⟦ dst ⇐ₛ v ⟧ C ⊢ ⟨fₜ @ pcₜ, j⟩ ≲ ⟨fₛ @ pc, S i⟩ {{ Q }} ->
+      C ⊢ ⟨fₜ @ pcₜ, j⟩ ≲ ⟨fₛ @ pcₛ, i⟩ {{ Q }}.
   Proof using Type.
-    intros pc dst op regs args v Hpc Hv [ρₜ mₜ] [ρₛ mₛ].
-    intros Harg Hsim. unfold_bilogic.
-    apply (@fsim_roll Λₜ Λₛ). subst.
+    intros pc dst op regs args v Hpc Hv.
+    intros ρₜ ρₛ mₜ mₛ Harg [? [Hnew Hsim]] Ψ Hpost. simp.
+
+    rewrite mapMtoMap in Harg.
+    injection Harg as Harg.
+
+    injection Hnew as Hnew.
+
     eapply FSourceSteps.
     - econstructor; eassumption || reflexivity.
-    - eapply (@fsim_unroll Λₜ Λₛ).
-      apply Hsim.
+    - now apply Hsim.
   Qed.
 
-  Lemma target_op iₜ iₛ fₜ fₛ pcₜ pcₛ :
+  Lemma target_op (C : Chain fsim_lfp) Q j fₜ pcₜ i fₛ pcₛ :
     ∀ pc dst op regs args v,
     fₜ@pcₜ is <{ dst := @op regs -> pc }> ->
     eval_op op args = Some v ->
-    ⊨ regs ↪ₜ args ->
-      ⟦ dst ↩ₜ v ⟧ (fₜ, pc) ⟨S iₜ ≲ iₛ⟩ (fₛ, pcₛ) {{ Φ }} ->
-      (fₜ, pcₜ) ⟨iₜ ≲ iₛ⟩ (fₛ, pcₛ) {{ Φ }}.
+    ⊨ regs ⇒ₜ args ->
+      ⟦ dst ⇐ₜ v ⟧ C ⊢ ⟨fₜ @ pc, S j⟩ ≲ ⟨fₛ @ pcₛ, i⟩ {{ Q }} ->
+      C ⊢ ⟨fₜ @ pcₜ, j⟩ ≲ ⟨fₛ @ pcₛ, i⟩ {{ Q }}.
   Proof using Type.
-    intros pc dst op regs args v Hpc Hv [ρₜ mₜ] [ρₛ mₛ].
-    intros Harg Hsim. unfold_bilogic.
-    apply (@fsim_roll Λₜ Λₛ). subst.
+    intros pc dst op regs args v Hpc Hv.
+    intros ρₜ ρₛ mₜ mₛ Harg [? [Hnew Hsim]] Ψ Hpost. simp.
+
+    rewrite mapMtoMap in Harg.
+    injection Harg as Harg.
+
+    injection Hnew as Hnew.
+
     eapply FTargetSteps.
     - eexists. econstructor; eassumption || reflexivity.
     - intros t Hstep. inv Hstep.
-      eexists.
-      eapply (@fsim_unroll Λₜ Λₛ).
-      apply Hsim.
+      eexists. now apply Hsim.
   Qed.
 
-  Lemma source_if iₜ iₛ fₜ fₛ pcₜ pcₛ :
-    ∀ pc_true pc_false reg v,
-    fₛ@pcₛ is <{ if reg then goto pc_true else goto pc_false }> ->
-    ⊨ reg ↪ₛ v ->
-      (fₜ, pcₜ) ⟨iₜ ≲ S iₛ⟩ (fₛ, if (v =? 0)%Z then pc_true else pc_false) {{ Φ }} ->
-      (fₜ, pcₜ) ⟨iₜ ≲ iₛ⟩ (fₛ, pcₛ) {{ Φ }}.
+  Lemma source_load (C : Chain fsim_lfp) Q j fₜ pcₜ i fₛ pcₛ :
+    ∀ pc dst src addr v,
+    fₛ@pcₛ is <{ dst := !src -> pc }> ->
+    ⊨ src ⇒ₛ addr ->
+      addr →ₛ v ->
+      ⟦ dst ⇐ₛ v ⟧ C ⊢ ⟨fₜ @ pcₜ, j⟩ ≲ ⟨fₛ @ pc, S i⟩ {{ Q }} ->
+      C ⊢ ⟨fₜ @ pcₜ, j⟩ ≲ ⟨fₛ @ pcₛ, i⟩ {{ Q }}.
   Proof using Type.
-    intros pc_true pc_false reg Hpc Hv [ρₜ mₜ] [ρₛ mₛ].
-    intros Harg Hsim. unfold_bilogic.
-    apply (@fsim_roll Λₜ Λₛ). subst.
+    intros pc dst src addr v Hpc.
+    intros ρₜ ρₛ mₜ mₛ Hsrc Haddr [? [Hnew Hsim]] Ψ Hpost. simp.
+
+    injection Hsrc as Hsrc.
+    injection Hnew as Hnew.
+
     eapply FSourceSteps.
     - econstructor; eassumption || reflexivity.
-    - eapply (@fsim_unroll Λₜ Λₛ).
-      apply Hsim.
+    - now eapply Hsim.
   Qed.
 
-  Lemma target_if iₜ iₛ fₜ fₛ pcₜ pcₛ :
-    ∀ pc_true pc_false reg v,
-    fₜ@pcₜ is <{ if reg then goto pc_true else goto pc_false }> ->
-    ⊨ reg ↪ₜ v ->
-      (fₜ, if (v =? 0)%Z then pc_true else pc_false) ⟨S iₜ ≲ iₛ⟩ (fₛ, pcₛ) {{ Φ }} ->
-      (fₜ, pcₜ) ⟨iₜ ≲ iₛ⟩ (fₛ, pcₛ) {{ Φ }}.
+  Lemma target_load (C : Chain fsim_lfp) Q j fₜ pcₜ i fₛ pcₛ :
+    ∀ pc dst src addr v,
+    fₜ@pcₜ is <{ dst := !src -> pc }> ->
+    ⊨ src ⇒ₜ addr ->
+      addr →ₜ v ->
+      ⟦ dst ⇐ₜ v ⟧ C ⊢ ⟨fₜ @ pc, S j⟩ ≲ ⟨fₛ @ pcₛ, i⟩ {{ Q }} ->
+      C ⊢ ⟨fₜ @ pcₜ, j⟩ ≲ ⟨fₛ @ pcₛ, i⟩ {{ Q }}.
   Proof using Type.
-    intros pc_true pc_false reg Hpc Hv [ρₜ mₜ] [ρₛ mₛ].
-    intros Harg Hsim. unfold_bilogic.
-    apply (@fsim_roll Λₜ Λₛ). subst.
+    intros pc dst src addr v Hpc.
+    intros ρₜ ρₛ mₜ mₛ Hsrc Haddr [? [Hnew Hsim]] Ψ Hpost. simp.
+
+    injection Hsrc as Hsrc.
+    injection Hnew as Hnew.
+
     eapply FTargetSteps.
     - eexists. econstructor; eassumption || reflexivity.
     - intros t Hstep. inv Hstep.
-      eexists.
-      eapply (@fsim_unroll Λₜ Λₛ).
-      apply Hsim.
+      eexists. now apply Hsim.
+  Qed.
+
+  Lemma source_store (C : Chain fsim_lfp) Q j fₜ pcₜ i fₛ pcₛ :
+    ∀ pc dst src addr v,
+    fₛ@pcₛ is <{ !dst := src -> pc }> ->
+    ⊨ src ⇒ₛ v ->
+      dst ⇒ₛ addr ->
+      ⟦ addr ←ₛ v ⟧ C ⊢ ⟨fₜ @ pcₜ, j⟩ ≲ ⟨fₛ @ pc, S i⟩ {{ Q }} ->
+      C ⊢ ⟨fₜ @ pcₜ, j⟩ ≲ ⟨fₛ @ pcₛ, i⟩ {{ Q }}.
+  Proof using Type.
+    intros pc dst src addr v Hpc.
+    intros ρₜ ρₛ mₜ mₛ Hsrc Haddr [? [Hnew Hsim]] Ψ Hpost. simp.
+
+    injection Hsrc as Hsrc.
+    injection Haddr as Haddr.
+
+    eapply FSourceSteps.
+    - econstructor; eassumption || reflexivity.
+    - now eapply Hsim.
+  Qed.
+
+  Lemma target_store (C : Chain fsim_lfp) Q j fₜ pcₜ i fₛ pcₛ :
+    ∀ pc dst src addr v,
+    fₜ@pcₜ is <{ !dst := src -> pc }> ->
+    ⊨ src ⇒ₜ v ->
+      dst ⇒ₜ addr ->
+      ⟦ addr ←ₜ v ⟧ C ⊢ ⟨fₜ @ pc, S j⟩ ≲ ⟨fₛ @ pcₛ, i⟩ {{ Q }} ->
+      C ⊢ ⟨fₜ @ pcₜ, j⟩ ≲ ⟨fₛ @ pcₛ, i⟩ {{ Q }}.
+  Proof using Type.
+    intros pc dst src addr v Hpc.
+    intros ρₜ ρₛ mₜ mₛ Hsrc Haddr [? [Hnew Hsim]] Ψ Hpost. simp.
+
+    injection Hsrc as Hsrc.
+    injection Haddr as Haddr.
+
+    eapply FTargetSteps.
+    - eexists. econstructor; eassumption || reflexivity.
+    - intros t Hstep. inv Hstep.
+      eexists. now apply Hsim.
+  Qed.
+
+  Lemma source_if (C : Chain fsim_lfp) Q j fₜ pcₜ i fₛ pcₛ :
+    ∀ pc_true pc_false reg v,
+    fₛ@pcₛ is <{ if reg then goto pc_true else goto pc_false }> ->
+    ⊨ reg ⇒ₛ v ->
+      C ⊢ ⟨fₜ @ pcₜ, j⟩ ≲ ⟨fₛ @ if (v =? 0)%Z then pc_true else pc_false, i⟩ {{ Q }} ->
+      C ⊢ ⟨fₜ @ pcₜ, j⟩ ≲ ⟨fₛ @ pcₛ, i⟩ {{ Q }}.
+  Proof using Type.
+    intros pc_true pc_false reg Hpc Hv.
+    intros ρₜ ρₛ mₜ mₛ Harg Hsim Ψ Hpost. simp.
+
+    injection Harg as Harg.
+
+    eapply FSourceSteps.
+    - econstructor; eassumption || reflexivity.
+    - now apply Hsim.
+  Qed.
+
+  Lemma target_if (C : Chain fsim_lfp) Q j fₜ pcₜ i fₛ pcₛ :
+    ∀ pc_true pc_false reg v,
+    fₜ@pcₜ is <{ if reg then goto pc_true else goto pc_false }> ->
+    ⊨ reg ⇒ₜ v ->
+      C ⊢ ⟨fₜ @ if (v =? 0)%Z then pc_true else pc_false, j⟩ ≲ ⟨fₛ @ pcₛ, i⟩ {{ Q }} ->
+      C ⊢ ⟨fₜ @ pcₜ, j⟩ ≲ ⟨fₛ @ pcₛ, i⟩ {{ Q }}.
+  Proof using Type.
+    intros pc_true pc_false reg Hpc Hv.
+    intros ρₜ ρₛ mₜ mₛ Harg Hsim Ψ Hpost. simp.
+
+    injection Harg as Harg.
+
+    eapply FTargetSteps.
+    - eexists. econstructor; eassumption || reflexivity.
+    - intros t Hstep. inv Hstep.
+      eexists. now apply Hsim.
   Qed.
 
 End Rules.
