theories/Commons/RegisterBank.v
@@ -1,0 +1,62 @@
+From RSL Require Import Prelude.
+
+From stdpp Require Import gmap.
+
+Definition reg := nat.
+
+(* [regmap] is a mapping from registers to a value *)
+Definition regbank : Type := gmap reg val.
+
+Definition get_reg (ρ: regbank) (r: reg) : val :=
+  match ρ !! r with
+  | Some v => v
+  | None => 0%Z (* Default val *)
+  end.
+
+Definition update_reg (ρ: regbank) (r: reg) (f: val -> val) : regbank :=
+  let old := get_reg ρ r in <[r := f old]>ρ.
+
+Canonical Structure regbank_ctx : LEnv :=
+  {|
+    get_data ρ r := Some $ get_reg ρ r;
+    update_data ρ r f := Some $ update_reg ρ r f;
+  |}.
+
+Definition set_reg (r: reg) (v: val) (ρ: regbank) : regbank :=
+  update_reg ρ r (fun _ => v).
+
+(* Fixpoint init_regs (vl: list val) (rl: list reg) : regbank := *)
+(*   match rl, vl with *)
+(*   | r :: rs, v :: vs => <[r := v]>(init_regs vs rs) *)
+(*   | _, _ => ∅ *)
+(*   end. *)
+
+(* Lemma get_regs_insert : ∀ regs r v ρ, *)
+(*   r ∉ regs -> *)
+(*   Forall (fun reg => get_reg (<[r := v]> ρ) reg = get_reg ρ reg) regs. *)
+(* Proof using Type. *)
+(*   intros regs r v ρ. *)
+(*   intros Hnotin. *)
+(*   induction regs as [ | r' regs IH]; constructor. *)
+(*   - unfold get_reg. rewrite (lookup_insert_ne ρ). *)
+(*     + reflexivity. *)
+(*     + intros ->. apply Hnotin. left. *)
+(*   - apply IH. intros Hin. apply Hnotin. now right. *)
+(* Qed. *)
+
+(* Lemma get_regs_init_regs : ∀ regs args, *)
+(*   NoDup regs -> *)
+(*   length args = length regs -> *)
+(*   get_regs (init_regs args regs) regs = args. *)
+(* Proof using Type. *)
+(*   intros regs args Hnodup. *)
+(*   revert args. *)
+(*   induction Hnodup as [|r regs Hnotin Hnodup IH]; intros args Hlen. *)
+(*   - destruct args; [reflexivity | discriminate Hlen]. *)
+(*   - destruct args as [|v args]; [discriminate Hlen |]. *)
+(*     simpl in Hlen. injection Hlen as Hlen'. *)
+(*     simpl. f_equal. *)
+(*     + unfold get_reg. now rewrite (lookup_insert_eq (init_regs args regs)). *)
+(*     + rewrite get_regs_insert by exact Hnotin. *)
+(*       apply IH. exact Hlen'. *)
+(* Qed. *)
