theories/Commons/Tactics.v
@@ -1,0 +1,10 @@
+From Ltac2 Require Import Ltac2 Printf.
+
+Ltac2 check (b: bool) : unit :=
+  match b with
+  | true => ()
+  | false => Control.zero (Tactic_failure (Some (fprintf "Check failed")))
+  end.
+
+Ltac2 print_goal () :=
+  Message.print (Message.of_constr (Control.goal ())).
