theories/RelLogic.v
@@ -1,0 +1,1 @@
+From RSL Require Export RelLogic.Logic.
