theories/RelLogic/Logic.v
@@ -1,0 +1,377 @@
+From RSL Require Import Prelude.
+
+(** ** Logic Definition  *)
+
+Definition rlogic (Et Es : LEnv) : Type :=
+  Et -> Es -> memory -> memory -> Prop.
+
+(* Notations scope *)
+Declare Scope rlogic_scope.
+Delimit Scope rlogic_scope with rlogic.
+Bind Scope rlogic_scope with rlogic.
+
+
+(** ** Logical Connectives *)
+
+Section LogicOp.
+  Context {Et Es: LEnv}.
+
+  Abbreviation rlogic := (rlogic Et Es).
+
+  Definition rlogic_and (P Q: rlogic) : rlogic :=
+    fun env_t env_s mt ms => P env_t env_s mt ms ∧ Q env_t env_s mt ms.
+
+  Definition rlogic_or (P Q: rlogic) : rlogic :=
+    fun env_t env_s mt ms => P env_t env_s mt ms ∨ Q env_t env_s mt ms.
+
+  Definition rlogic_impl (P Q: rlogic) : rlogic :=
+    fun env_t env_s mt ms => P env_t env_s mt ms -> Q env_t env_s mt ms.
+
+  Definition rlogic_not (P: rlogic) : rlogic :=
+    fun env_t env_s mt ms => ~ P env_t env_s mt ms.
+
+  Definition rlogic_exists {X: Type} (f: X -> rlogic) : rlogic :=
+    fun env_t env_s mt ms => ∃ x, f x env_t env_s mt ms.
+
+  Definition rlogic_forall {X: Type} (f: X -> rlogic) : rlogic :=
+    fun env_t env_s mt ms => ∀ x, f x env_t env_s mt ms.
+
+  Definition rlogic_pure (P: Prop) : rlogic :=
+    fun _ _ _ _ => P.
+
+  Definition rlogic_memory_pure (P: memory -> memory -> Prop) : rlogic :=
+    fun _ _ mt ms => P mt ms.
+
+  Definition rlogic_env_t_pure (P: Et -> Prop) : rlogic :=
+    fun env_t _ _ _  => P env_t.
+
+  Definition rlogic_env_s_pure (P: Es -> Prop) : rlogic :=
+    fun _ env_s _ _  => P env_s.
+
+  Definition rlogic_entails (P: rlogic) : Prop :=
+    ∀ env_t env_s mt ms, P env_t env_s mt ms.
+
+  Global Instance top_rlogic : Top rlogic := rlogic_pure True.
+  Global Instance bot_rlogic : Bottom rlogic := rlogic_pure False.
+
+End LogicOp.
+
+Notation "x ∧ y" :=
+  (rlogic_and x y)
+    (at level 80, y constr at level 80, right associativity) : rlogic_scope.
+
+Notation "x ∨ y" :=
+  (rlogic_or x y)
+    (at level 85, y constr at level 85, right associativity) : rlogic_scope.
+
+Notation "x → y" := (rlogic_impl x y)
+  (at level 99, y at level 200, right associativity) : rlogic_scope.
+
+Notation "x -> y" := (rlogic_impl x y)
+  (at level 99, y at level 200, right associativity) : rlogic_scope.
+
+Notation "~ x" :=
+  (rlogic_not x)
+    (at level 75, x constr at level 75, right associativity) : rlogic_scope.
+
+Notation "¬ x" :=
+  (rlogic_not x)
+    (at level 75, x constr at level 75, right associativity) : rlogic_scope.
+
+Notation "∀ x .. y , P" :=
+  (rlogic_forall (fun x => .. (rlogic_forall (fun y => P)) ..))
+    (at level 10, x binder, y binder, P at level 200,
+     format "'[ ' '[ ' ∀ x .. y ']' , '/' P ']'") : rlogic_scope.
+
+Notation "∃ x .. y , P" :=
+  (rlogic_exists (fun x => .. (rlogic_exists (fun y => P)) ..))
+    (at level 10, x binder, y binder, P at level 200,
+     format "'[ ' '[ ' ∃ x .. y ']' , '/' P ']'") : rlogic_scope.
+
+Notation "⌜ P ⌝" :=
+  (rlogic_pure P) (at level 0, format "⌜ P ⌝") : rlogic_scope.
+
+Notation "⌜ P ⌝ₘ" :=
+  (rlogic_memory_pure P) (at level 0, format "⌜ P ⌝ₘ") : rlogic_scope.
+
+Notation "⌜ P ⌝ₜ" :=
+  (rlogic_env_t_pure P) (at level 0, format "⌜ P ⌝ₜ") : rlogic_scope.
+
+Notation "⌜ P ⌝ₛ" :=
+  (rlogic_env_s_pure P) (at level 0, format "⌜ P ⌝ₛ") : rlogic_scope.
+
+Notation "⦇ P ⦈" :=
+  (P)%rlogic (at level 0, P at level 200, format "⦇ P ⦈").
+
+Notation "⊨ P" :=
+  (rlogic_entails P%rlogic) (at level 99, right associativity).
+
+Notation "'True'" := (rlogic_pure True) (format "True") : rlogic_scope.
+Notation "'False'" := (rlogic_pure False) (format "False") : rlogic_scope.
+
+
+(** ** Memory Connectives *)
+
+Section MemoryOp.
+  Context {Et Es: LEnv}.
+
+  Abbreviation rlogic := (rlogic Et Es).
+
+  Definition rlogic_mem_t_assert addr v : rlogic :=
+    fun _ _ mt _ => get_at addr mt = Some v.
+
+  Definition rlogic_mem_s_assert addr v : rlogic :=
+    fun _ _ _ ms => get_at addr ms = Some v.
+
+  Definition rlogic_mem_t_set addr v (P: rlogic) : rlogic :=
+    fun env_t env_s mt ms =>
+      ∃ mt', set_at addr v mt = Some mt' ∧ P env_t env_s mt' ms.
+
+  Definition rlogic_mem_s_set addr v (P: rlogic) : rlogic :=
+    fun env_t env_s mt ms =>
+      ∃ ms', set_at addr v ms = Some ms' ∧ P env_t env_s mt ms'.
+
+  Definition rlogic_mem_same_at P addrt addrs : rlogic :=
+    fun _ _ mt ms =>
+      P (get_at addrt mt) (get_at addrs ms).
+
+End MemoryOp.
+
+(* Global Strategy opaque *)
+(*   [ *)
+(*     rlogic_mem_t_assert *)
+(*     rlogic_mem_s_assert *)
+(*     rlogic_mem_t_set *)
+(*     rlogic_mem_s_set *)
+(*     rlogic_mem_at_same *)
+(*   ]. *)
+
+Notation "l '→ₜ' v" :=
+  (rlogic_mem_t_assert l%positive v%Z)
+    (at level 70, no associativity, format "l →ₜ v") : rlogic_scope.
+
+Notation "l '→ₛ' v" :=
+  (rlogic_mem_s_assert l%positive v%Z)
+    (at level 70, no associativity, format "l →ₛ v") : rlogic_scope.
+
+Notation "'⟦' addr '←ₜ' v '⟧' P" :=
+  (rlogic_mem_t_set addr%positive v%Z P)
+    (at level 20, P at level 20, right associativity).
+
+Notation "'⟦' addr '←ₛ' v '⟧' P" :=
+  (rlogic_mem_s_set addr%positive v%Z P)
+    (at level 20, P at level 20, right associativity).
+
+Notation "'⟦' addrt '←ₜ' vt ',' addrs '←ₛ' vs '⟧' P" :=
+  (rlogic_mem_t_set addrt%positive vt%Z
+     (rlogic_mem_s_set addrs%positive vs%Z P))
+    (at level 20, P at level 20, right associativity).
+
+Notation "'⟦' addrs '←ₛ' vs ',' addrt '←ₜ' vt '⟧' P" :=
+  (rlogic_mem_t_set addrt%positive vt%Z
+     (rlogic_mem_s_set addrs%positive vs%Z P))
+    (at level 20, P at level 20, right associativity).
+
+Notation "addrt 'ₜ⟨' P '⟩ₛ' addrs" :=
+  (rlogic_mem_same_at P addrt%positive addrs%positive)
+    (at level 70, no associativity) : rlogic_scope.
+
+Notation "addrs 'ₛ⟨' P '⟩ₜ' addrt" :=
+  (rlogic_mem_same_at P addrt%positive addrs%positive)
+    (at level 70, no associativity) : rlogic_scope.
+
+Notation "addrt 'ₜ~ₛ' addrs" :=
+  (rlogic_mem_same_at eq addrt%positive addrs%positive)
+    (at level 70, no associativity) : rlogic_scope.
+
+Notation "addrs 'ₛ~ₜ' addrt" :=
+  (rlogic_mem_same_at eq addrt%positive addrs%positive)
+    (at level 70, no associativity) : rlogic_scope.
+
+
+(** ** Target Context Connectives *)
+
+Section TargetOp.
+  Context {Et Es: LEnv}.
+
+  Abbreviation rlogic := (rlogic Et Es).
+
+  Class RLogicTargetAssert (R V : Type) :=
+    rlogic_env_t_assert : R -> V -> rlogic.
+
+  Global Instance rlogic_env_t_assert_single : RLogicTargetAssert _ _ :=
+    fun key val env_t _ _ _ =>
+      get_data env_t key = Some val.
+
+  Global Instance rlogic_env_t_assert_list : RLogicTargetAssert (list _) (list _) :=
+    fun keys vals env_t _ _ _ =>
+      mapM (get_data env_t) keys = Some vals.
+
+  Definition rlogic_env_t_update key f (P : rlogic) : rlogic :=
+    fun env_t env_s mt ms =>
+      ∃ env_t',
+        update_data env_t key f = Some env_t' ∧
+        P env_t' env_s mt ms.
+
+  Definition rlogic_env_t_set key val (P : rlogic) : rlogic :=
+    rlogic_env_t_update key (fun _ => val) P.
+
+End TargetOp.
+
+(* Global Strategy opaque *)
+(*   [ *)
+(*     rlogic_env_t_assert *)
+(*     rlogic_env_t_assert_helper *)
+(*     rlogic_env_t_assert_single *)
+(*     rlogic_env_t_assert_list *)
+(*     rlogic_env_t_update *)
+(*     rlogic_env_t_set *)
+(*   ]. *)
+
+Notation "r '⇒ₜ' v" :=
+  (rlogic_env_t_assert r%nat v%Z)
+    (at level 70, no associativity, format "r ⇒ₜ v").
+
+Notation "'⟦' r '⇐ₜ' v '⟧' P" :=
+  (rlogic_env_t_set r%nat v%Z P)
+    (at level 20, P at level 20, right associativity).
+
+Notation "'⟦' r '⇐ₜ' 'λ' v '.' f '⟧' P" :=
+  (rlogic_env_t_update r%nat (fun v => f) P)
+    (at level 20, v binder, P at level 20, right associativity).
+
+Notation "'⟦' r '⇐ₜ' 'fun' v '.' f '⟧' P" :=
+  (rlogic_env_t_update r%nat (fun v => f) P)
+    (at level 20, v binder, P at level 20, right associativity).
+
+
+(** ** Source Context Connectives *)
+
+Section SourceOp.
+  Context {Et Es: LEnv}.
+
+  Abbreviation rlogic := (rlogic Et Es).
+
+  Class RLogicSourceAssert (R V : Type) :=
+    rlogic_env_s_assert : R -> V -> rlogic.
+
+  Global Instance rlogic_env_s_assert_single : RLogicSourceAssert _ _ :=
+    fun key val _ env_s _ _ =>
+      get_data env_s key = Some val.
+
+  Global Instance rlogic_env_s_assert_list : RLogicSourceAssert (list _) (list _) :=
+    fun keys vals _ env_s _ _ =>
+      mapM (get_data env_s) keys = Some vals.
+
+  Definition rlogic_env_s_update key f (P : rlogic) : rlogic :=
+    fun env_t env_s mt ms =>
+      ∃ env_s',
+        update_data env_s key f = Some env_s' ∧
+        P env_t env_s' mt ms.
+
+  Definition rlogic_env_s_set key val (P : rlogic) : rlogic :=
+    rlogic_env_s_update key (fun _ => val) P.
+
+End SourceOp.
+
+(* Global Strategy opaque *)
+(*   [ *)
+(*     rlogic_env_s_assert *)
+(*     rlogic_env_s_assert_helper *)
+(*     rlogic_env_s_assert_single *)
+(*     rlogic_env_s_assert_list *)
+(*     rlogic_env_s_update *)
+(*     rlogic_env_s_set *)
+(*   ]. *)
+
+Notation "r '⇒ₛ' v" :=
+  (rlogic_env_s_assert r%nat v%Z)
+    (at level 70, no associativity, format "r ⇒ₛ v").
+
+Notation "'⟦' r '⇐ₛ' v '⟧' P" :=
+  (rlogic_env_s_set r%nat v%Z P)
+    (at level 20, P at level 20, right associativity).
+
+Notation "'⟦' r '⇐ₛ' 'λ' v '.' f '⟧' P" :=
+  (rlogic_env_s_update r%nat (fun v => f) P)
+    (at level 20, v binder, P at level 20, right associativity).
+
+Notation "'⟦' r '⇐ₛ' 'fun' v '.' f '⟧' P" :=
+  (rlogic_env_s_update r%nat (fun v => f) P)
+    (at level 20, v binder, P at level 20, right associativity).
+
+(** ** Both Context Connectives *)
+
+Section BothLEnvOp.
+  Context {Et Es: LEnv}.
+
+  Abbreviation rlogic := (rlogic Et Es).
+
+  Definition rlogic_env_same_at P keyt keys : rlogic :=
+    fun env_t env_s _ _ =>
+      P (get_data env_t keyt) (get_data env_s keys).
+
+End BothLEnvOp.
+
+Notation "'⟦' rt '⇐ₜ' vt ',' rs '⇐ₛ' vs '⟧' P" :=
+  (rlogic_env_t_set rt%nat vt%Z (rlogic_env_s_set rs%nat vs%Z P))
+    (at level 20, P at level 20, right associativity).
+
+Notation "'⟦' rs '⇐ₛ' vs ',' rt '⇐ₜ' vt '⟧' P" :=
+  (rlogic_env_t_set rt%nat vt%Z (rlogic_env_s_set rs%nat vs%Z P))
+    (at level 20, P at level 20, right associativity).
+
+Notation "rt 'ₜ⟪' P '⟫ₛ' rs" :=
+  (rlogic_env_same_at P rt%nat rs%nat)
+    (at level 70, no associativity) : rlogic_scope.
+
+Notation "rs 'ₛ⟪' P '⟫ₜ' rt" :=
+  (rlogic_env_same_at P rt%nat rs%nat)
+    (at level 70, no associativity) : rlogic_scope.
+
+Notation "rt 'ₜ≈ₛ' rs" :=
+  (rlogic_env_same_at eq rt%nat rs%nat)
+    (at level 70, no associativity) : rlogic_scope.
+
+Notation "rs 'ₛ≈ₜ' rt" :=
+  (rlogic_env_same_at eq rt%nat rs%nat)
+    (at level 70, no associativity) : rlogic_scope.
+
+(** ** Auto unfolding *)
+
+Create HintDb custom_rlogic discriminated.
+
+Hint Unfold
+  rlogic_and
+  rlogic_or
+  rlogic_impl
+  rlogic_not
+  rlogic_exists
+  rlogic_forall
+
+  rlogic_pure
+  rlogic_memory_pure
+  rlogic_env_t_pure
+  rlogic_env_s_pure
+
+  rlogic_entails
+
+  rlogic_mem_t_assert
+  rlogic_mem_s_assert
+  rlogic_mem_same_at
+
+  rlogic_env_t_assert
+  rlogic_env_t_assert_single
+  rlogic_env_t_assert_list
+
+  rlogic_env_s_assert
+  rlogic_env_s_assert_single
+  rlogic_env_s_assert_list
+
+  rlogic_env_same_at
+
+  get_data : custom_rlogic.
+
+Ltac simp :=
+  autounfold with custom_rlogic in *;
+  cbn beta iota zeta delta in *.
