theories/Simulations/FreeSimRules.v
@@ -1,0 +1,105 @@
+From RSL Require Import Prelude.
+
+From Coinduction Require Import all.
+
+From RSL Require Import Simulations.Commons.
+From RSL Require Import Simulations.FreeSim.
+From RSL Require Import Simulations.Equiv.
+
+Section FSimRules.
+  Context {Λₜ Λₛ: lang}.
+  Context (J I: WfRel).
+  Context (Pₜ: prog Λₜ) (Pₛ: prog Λₛ).
+
+  Abbreviation fsim := (fsim J I Pₜ Pₛ).
+  Abbreviation fsim_lfp := (fsim_lfp J I Pₜ Pₛ).
+
+  Lemma fsim_in_chain Φ:
+    ∀ j t i s,
+    (∀ R : Chain fsim_lfp, fsim_lfp (elem R) Φ j t i s) ->
+    fsim Φ j t i s.
+  Proof using Type.
+    intros j t i s Hr.
+    unfold fsim.
+    apply (gfp_prop).
+    intros C.
+    apply (b_chain C), Hr.
+  Qed.
+
+  Lemma final (C: Chain fsim_lfp) Φ:
+    ∀ j t i s,
+    are_final Φ t s ->
+    fsim_lfp (elem C) Φ j t i s.
+  Proof using Type.
+    apply tower.
+    { intros P Hp j t i s H Q Hq. eapply Hp; now eauto. }
+    intros C' CIH j t i s H. econstructor; now eauto.
+  Qed.
+
+  Lemma stuck (C: Chain fsim_lfp) Φ:
+    ∀ j t i s,
+    stuck Pₛ s ->
+    fsim_lfp (elem C) Φ j t i s.
+  Proof using Type.
+    apply tower.
+    { intros P Hp j t i s H Q Hq. eapply Hp; now eauto. }
+    intros C' CIH j t i s H. econstructor; now eauto.
+  Qed.
+
+  Lemma source_step (C: Chain fsim_lfp) Φ:
+    ∀ j t i i' s s',
+    Pₛ ⊨ s ->> s' ->
+    fsim_lfp (elem C) Φ j t i' s' ->
+    fsim_lfp (elem C) Φ j t i s.
+  Proof using Type.
+    apply tower.
+    { intros P Hp j t i i' s s' Hstep H Q Hq. eapply Hp; now eauto. }
+    intros C' CIH j t i i' s s' Hstep H. econstructor; now eauto.
+  Qed.
+
+  Lemma target_step (C: Chain fsim_lfp) Φ:
+    ∀ j t i s,
+    can_progress Pₜ t ->
+    (∀ t', Pₜ ⊨ t ->> t' -> ∃ j', fsim_lfp (elem C) Φ j' t' i s) ->
+    fsim_lfp (elem C) Φ j t i s.
+  Proof using Type.
+    apply tower.
+    { intros P Hp j t i s Hprogesss H Q Hq.
+      eapply Hp; eauto.
+      intros t' Hstep. destruct (H _ Hstep) as [j' Hinf].
+      exists j'. now auto. }
+    intros C' CIH j t i s Hprogress Ht. econstructor; now eauto.
+  Qed.
+
+  Lemma progress_step (C: Chain fsim_lfp) Φ:
+    ∀ j j' t i i' s,
+    j' ⊏ j ->
+    i' ⊏ i ->
+    fsim_lfp (elem C) Φ j' t i' s ->
+    fsim_lfp (elem C) Φ j t i s.
+  Proof using Type.
+    apply tower.
+    { intros P Hp j j' t i i' s Ht Hs H Q Hq.
+      eapply Hp; now eauto. }
+    intros C' CIH j j' t i i' s Ht Hs H.
+    eapply FProgress; try eassumption.
+    now apply (b_chain C').
+  Qed.
+
+  Lemma coind_rule (C: Chain fsim_lfp) Φ:
+    ∀ t s,
+    (∀ C': Chain fsim_lfp,
+       ∀ j i,
+       (∀ j' i', (elem C') Φ j' t i' s) ->
+       fsim_lfp (elem C') Φ j t i s) ->
+    ∀ j i, fsim_lfp (elem C) Φ j t i s.
+  Proof using Type.
+    intros t s RIH.
+    apply tower.
+    { intros P Hp j i Q Hq. eapply Hp; now eauto. }
+    intros C' CIH j i.
+    eapply fsim_lfp'_mono with (x := fun j t i s => (elem C') j t i s).
+    - intros Ψ j' t' i' s' Hc. assumption.
+    - eapply RIH; try eassumption.
+  Qed.
+End FSimRules.
