theories/Toy/Toy.v
@@ -1,5 +1,9 @@
 From RSL Require Import Prelude.
 
+From RSL Require Export Commons.RegisterBank.
+
+From stdpp Require Import strings.
+
 Variant texpr : Type :=
 | EReg (r: reg)
 | EImm (v: val)
@@ -12,7 +16,7 @@ Inductive tinstr : Type :=
 | ISkip
 | IBreak (level: nat)
 | IRet (v: reg)
-| ICall (dst: reg) (name: ident) (args: list reg)
+| ICall (dst: reg) (name: string) (args: list reg)
 | ISeq (fst snd: tinstr)
 | IAssign (dst: reg) (e: texpr)
 | IStore  (addr: reg) (e: reg)
@@ -26,7 +30,7 @@ Definition IDoWhile (body: tinstr) (cond: reg) : tinstr :=
   ILoop (ISeq body (IIf cond ISkip (IBreak 0))) ISkip.
 
 Record tfunction := {
-    tfn_name: ident;
+    tfn_name: string;
     tfn_regs: list reg;
     tfn_code : tinstr;
     tfn_regs_no_dup : is_no_dup tfn_regs = true;
