theories/Prelude/LogicEnv.v
@@ -1,0 +1,17 @@
+(** ** Custom context structure *)
+
+Structure LEnv := {
+    (** Environment type with coercion. *)
+    E :> Type;
+    (** Keys *)
+    Key : Type;
+    (** Values *)
+    Val : Type;
+    (** Get handler  *)
+    get_data : E -> Key -> option Val;
+    (** Update handler *)
+    update_data : E -> Key -> (Val -> Val) -> option E;
+}.
+
+Arguments get_data {_} _ _.
+Arguments update_data {_} _ _ _.
